case_studies/HamiltonBlum/Blum_Completeness.ec
@@ -7,6 +7,7 @@ require import Permutation Blum_Basics.
 
 section.
 
+
 local lemma hc_complete_hoare pa wa : IsHC (pa,wa) =>
    hoare[ Completeness(HonestProver, HV).run : arg = (pa,wa) ==> res ].
 move => ishc. proc. inline*. wp. rnd. 
@@ -16,23 +17,23 @@ pose b1 := ch.
 
 case (b1 = true). 
 move => h. rewrite h. simplify.
-  + have ->: (zip (unzip1 x0) (unzip2 x0)) = x0. rewrite zip_unzip. auto.
+  + have ->: (zip (unzip1 pi_gwco) (unzip2 pi_gwco)) = pi_gwco. rewrite zip_unzip. auto.
 split.
 have : all (fun (xy : bool * (commitment * opening) ) => xy.`2 \in (Com xy.`1)) 
-    (zip  (permute_graph prm s{hr}.`2) x0).
+    (zip  (permute_graph prm s{hr}) pi_gwco).
 have f3 :   
-  size (permute_graph prm s{hr}.`2) = size x0 /\
+  size (permute_graph prm s{hr}) = size pi_gwco /\
   all (fun (xy : bool * (commitment * opening)) => xy.`2 \in Com xy.`1)
-    (zip (permute_graph prm s{hr}.`2) x0).
-apply (supp_djoinmap Com ((permute_graph prm s{hr}.`2))  x0). auto.
+    (zip (permute_graph prm s{hr}) pi_gwco).
+apply (supp_djoinmap Com ((permute_graph prm s{hr}))  pi_gwco). auto.
 elim f3. move => f31 f32.
 auto.
 move => q.
 apply (sub_all (fun (xy : bool * (commitment * opening)) => xy.`2 \in Com xy.`1) Ver) .
 simplify. apply Com_sound.  auto.
-have f1 : size x0 = size (permute_graph prm s{hr}.`2).
+have f1 : size pi_gwco = size (permute_graph prm s{hr}).
 smt.
-have f2 : size x0 = size (unzip1 x0).
+have f2 : size pi_gwco = size (unzip1 pi_gwco).
 smt.
 rewrite - f2. 
 rewrite f1.
@@ -41,101 +42,73 @@ split. smt. split. smt. smt.
 move => p.
 have ->: b1 = false. smt.
 simplify. clear p. progress.
-apply (kjk prm s{hr}.`1). auto. smt (ishc_prop4). smt (ishc_prop4).
-smt. 
-smt.
-have ->: size (unzip1 x0) = size x0. smt.
-have -> : size x0 = size (permute_graph prm s{hr}.`2). smt(supp_djoinmap).
-have -> : size (permute_graph prm s{hr}.`2) = size (s{hr}.`2). smt. smt.
-have ->: size (unzip2 (take s{hr}.`1 (ip (prj (permute_witness prm w{hr})) x0)))
- = size (take s{hr}.`1 (ip (prj (permute_witness prm w{hr})) x0)). smt.
-have : s{hr}.`1 <= size (ip (prj (permute_witness prm w{hr})) x0).
-have ->: size (ip (prj (permute_witness prm w{hr})) x0) = size x0.
-smt.
-have -> : size x0 = size (permute_graph prm s{hr}.`2). smt(supp_djoinmap).
-have -> : size (permute_graph prm s{hr}.`2) = size (s{hr}.`2). smt. timeout 20. smt.
-progress. smt.
+apply (kjk prm ). auto. 
+
+elim ishc. smt.
+smt.  smt.
+have : size pi_gwco = size (permute_graph prm s{hr}). smt.
+have ->: size (permute_graph prm s{hr}) = size s{hr}. smt. 
+have ->: size s{hr} = K * K. elim ishc. smt.
+move => q. 
+have qqq : size (prj_path (permute_witness prm w{hr}) pi_gwco) = K.
+smt. smt.
+
+(* have ->: size (unzip1 x0) = size x0. smt. *)
+(* have -> : size x0 = size (permute_graph prm s{hr}). smt(supp_djoinmap). *)
+(* have -> : size (permute_graph prm s{hr}) = size (s{hr}). smt. smt. *)
+
+
+(* have : size (prj_path (permute_witness prm w{hr}) x0) = K. *)
+(*    have ->: K = size (permute_witness prm w{hr}). smt. *)
+(* apply (lemma1 (permute_witness prm w{hr}) x0).  *)
+(*   have -> : size (permute_witness prm w{hr}) = size w{hr}. smt. *)
+(* have -> : size x0 = size (permute_graph prm s{hr}). smt(supp_djoinmap). *)
+(* have -> : size (permute_graph prm s{hr}) = size (s{hr}). smt.  *)
+(* elim ishc. smt. *)
+(* smt. *)
+
+have ->: (prj_path (permute_witness prm w{hr}) (unzip1 pi_gwco))
+  = (unzip1 (prj_path (permute_witness prm w{hr}) pi_gwco)).
+rewrite lemma2. auto.
+
 have ->: 
-  (unzip2 (take s{hr}.`1 (ip (prj (permute_witness prm w{hr})) x0)))
-  = ((take s{hr}.`1 (unzip2 (ip (prj (permute_witness prm w{hr})) x0)))).
-smt.
-have ->: 
-  (zip (take s{hr}.`1 (ip (prj (permute_witness prm w{hr})) (unzip1 x0)))
-     (take s{hr}.`1 (unzip2 (ip (prj (permute_witness prm w{hr})) x0))))
-  = take s{hr}.`1  
-     (zip ((ip (prj (permute_witness prm w{hr})) (unzip1 x0)))
-          ((unzip2 (ip (prj (permute_witness prm w{hr})) x0)))).
-apply take_zip.
-have ->: ((ip (prj (permute_witness prm w{hr})) (unzip1 x0)))
-  = (unzip1 (ip (prj (permute_witness prm w{hr})) (x0))).
-rewrite map_ip. auto.
-have ->: 
- (zip (unzip1 (ip (prj (permute_witness prm w{hr})) x0))
-        (unzip2 (ip (prj (permute_witness prm w{hr})) x0)))
- = (ip (prj (permute_witness prm w{hr})) x0).
+ (zip (unzip1 (prj_path (permute_witness prm w{hr}) pi_gwco))
+        (unzip2 (prj_path (permute_witness prm w{hr}) pi_gwco)))
+ = ((prj_path (permute_witness prm w{hr}) pi_gwco)). 
 apply zip_unzip.
-pose pi_w := (permute_witness prm w{hr}).
-pose n := s{hr}.`1.
-pose permute_graphg := (permute_graph prm s{hr}.`2). 
-have ->: 
- all Ver (zip (nseq n true) (take n (ip (prj pi_w) x0)))
- = all (fun x => Ver x)
-  (take n (zip (nseq n true) (ip (prj pi_w) x0))).
-rewrite - take_zip.
-rewrite take_nseq. auto.
-have ->: (take n (zip (nseq n true) (ip (prj pi_w) x0))) =
-  (take n (zip (ip (prj pi_w) permute_graphg) (ip (prj pi_w) x0))).
-  have ->: take n (zip (nseq n true) (ip (prj pi_w) x0)) =
-     (zip (nseq n true) (ip (prj pi_w) x0)). 
-apply take_oversize.
-rewrite size_zip.
-rewrite size_nseq. 
-  have ->: (max 0 n) = n.  smt(ishc_prop2). smt.
-  have ->: take n (zip (ip (prj pi_w) permute_graphg) (ip (prj pi_w) x0))
-   = (zip (take n (ip (prj pi_w) permute_graphg)) (take n (ip (prj pi_w) x0))).
-   rewrite - take_zip. auto.
-  have ->: (take n (ip (prj pi_w) permute_graphg)) = nseq n true.
-  rewrite - (ishc_prop3 (s{hr}, w{hr}) s{hr}.`1 s{hr}.`2 w{hr}). auto. smt. rewrite /n.
-  have ->: s{hr}.`1 = size (w{hr}). smt. rewrite -  prj_lemma. auto.   
-rewrite - take_nseq.
-rewrite take_zip.
-rewrite take_nseq.
-rewrite take_oversize.
-rewrite size_zip.
-rewrite size_nseq. 
-  have ->: (max 0 n) = n.  smt(ishc_prop2). smt.
-auto.   
-have f1 : all Ver (zip permute_graphg x0). 
-search djoin.
-  have :   size (permute_graph prm s{hr}.`2) = size x0 /\ all (fun xy => snd xy \in Com xy.`1) (zip permute_graphg x0).
-   apply (supp_djoinmap Com permute_graphg x0 ). apply H0.
-   elim. progress.
-  have : forall x, x \in (zip permute_graphg x0) => x.`2 \in Com x.`1.
-apply allP. apply H3.
-progress.
-apply allP. progress. 
-  have : x1.`2 \in Com x1.`1. apply H4. auto.
-  apply Com_sound.
-have f2 : all Ver (zip (ip (prj pi_w) permute_graphg)  (ip (prj pi_w) x0)).
-rewrite - zip_ip.
-have : forall x, x \in (zip permute_graphg x0) => Ver x.
-apply allP. apply f1.
-progress.
-have : forall x, x \in (ip (prj pi_w) (zip permute_graphg x0)) => Ver x.
-progress. apply H2.
-  have ff : perm_eq (zip permute_graphg x0) (ip (prj pi_w) (zip permute_graphg x0)).
-   smt.
-  smt.
-apply allP.
-timeout 20. smt.
-rewrite /permute_witness.
 elim ishc. progress.
-have : perm_eq (map prm w{hr}) (map prm (range 0 s{hr}.`1)).
-smt.
+
+apply allP.
+move => x1.
+
+have ->: (nseq K true) = (prj_path (permute_witness prm w{hr}) (permute_graph prm s{hr})).
+rewrite  (lemma3  (permute_witness prm w{hr}) (permute_graph prm s{hr})). apply lemma4. auto. auto.
 progress.
-have : perm_eq (map prm (range 0 s{hr}.`1)) (range 0 s{hr}.`1).
+apply Com_sound.
+
+
+
+have : x1.`1 \in (nseq K true). smt.
+progress.
+have : x1.`2 \in (prj_path (permute_witness prm w{hr}) pi_gwco).
+   smt.
+ move => qq.
+have : x1.`2 \in pi_gwco. apply (lemma5 x1.`2 (permute_witness prm w{hr})). auto.
+move => qqq.
+
+  have :   size (permute_graph prm s{hr}) = size pi_gwco /\ all (fun xy => snd xy \in Com xy.`1) (zip (permute_graph prm s{hr}) pi_gwco).
+   apply (supp_djoinmap Com (permute_graph prm s{hr}) pi_gwco ). apply H0.
+   elim. progress.
+  have : forall x, x \in (zip (permute_graph prm s{hr}) pi_gwco) => x.`2 \in Com x.`1.
+apply allP. apply H9.
+progress. apply H10. 
+  have z : x1.`1 \in (prj_path (permute_witness prm w{hr}) (permute_graph prm s{hr})). smt.
+  have z2 : x1.`1 \in (permute_graph prm s{hr}). smt (lemma5).
+have ->: x1 = (x1.`1,x1.`2). smt.
+apply (lemma6 x1.`1 (permute_graph prm s{hr}) x1.`2 pi_gwco).
 smt.
-smt.
+auto. auto. 
+smt(lemma7 perm_eq_trans).
 smt.
 qed.
 
