case_studies/HamiltonBlum/Blum_ZeroKnowledge.ec
@@ -1,0 +1,66 @@
+pragma Goals:printall.
+require import AllCore DBool Bool List Distr Int Aux DJoin.
+require import Permutation Blum_Basics Blum_Sim1Property.
+
+import DJMM.
+import OSS.
+
+clone import Statistical with op epsilon <- 2%r * negl + 20%r * negl2,
+                              op sigma <- (1%r/2%r - negl2).
+
+
+
+require RewBasics.
+clone import RewBasics as Rew with type sbits <- sbits.
+
+
+section.
+
+declare module V <: RewMaliciousVerifier{-HonestProver, -ZKT.Hyb.HybOrcl,-ZKT.Hyb.Count, -HP'}.
+declare module D <: ZKDistinguisher{-HonestProver, -V, -ZKT.Hyb.HybOrcl,-ZKT.Hyb.Count, -HP' }.
+
+
+declare axiom Sim1_run_ll : forall (V0 <: RewMaliciousVerifier), islossless V0.challenge => islossless V0.summitup => islossless Sim1(V0).run.
+declare axiom V_summitup_ll : islossless V.summitup. 
+declare axiom V_challenge_ll : islossless V.challenge.
+declare axiom D_guess_ll : islossless D.guess.
+declare axiom P_response_ll : islossless HonestProver.response.
+declare axiom P_commitment_ll : islossless HonestProver.commitment.
+
+declare axiom D_guess_prop : equiv[ D.guess ~ D.guess : ={glob V, arg} ==> ={res} ].
+
+declare axiom rewindable_V_plus :
+        (exists (f : glob V -> sbits),
+         injective f /\
+         (forall &m, Pr[ V.getState() @ &m : (glob V) = ((glob V){m})
+                                               /\ res = f ((glob V){m}) ] = 1%r) /\
+         (forall &m b (x: glob V), b = f x =>
+           Pr[V.setState(b) @ &m : glob V = x] = 1%r) /\
+         islossless V.setState).
+
+
+lemma hc_statistical_zk stat wit  &m:
+        zk_relation stat wit => 
+        let real_prob = Pr[ZKReal(HonestProver, V, D).run(stat, wit) @ &m : res] in
+        let ideal_prob = Pr[ZKIdeal(SimN(Sim1), V, D).run(stat, wit) @ &m : res] in
+          `|ideal_prob - real_prob| <= (2%r * negl + 20%r * negl2) + 2%r * (1%r- (1%r/2%r - negl2)) ^ OSS.N.
+proof.
+progress.
+apply (statistical_zk HonestProver Sim1  V D _ _ _ _ _ _ _ _ _ _  stat wit &m _). apply Sim1_run_ll. apply V_summitup_ll. apply V_challenge_ll. apply P_response_ll. apply P_commitment_ll.
+apply D_guess_ll. 
+proc*. call D_guess_prop. skip.  auto.
+move => x.
+apply (sim1_rew_ph V _ _ _ _ _ x). apply V_summitup_ll. apply V_challenge_ll. apply P_response_ll. apply P_commitment_ll.
+apply (rewindable_A_plus V). apply rewindable_V_plus.
+progress.
+apply (sim1_prop V D  _ _  _ _ _  &m0 p w  _ );auto.  apply V_summitup_ll. apply (rewindable_A_plus V). apply rewindable_V_plus. 
+apply D_guess_ll. apply V_summitup_ll. apply V_challenge_ll. 
+progress.
+apply (sim1assc V D _ _ _ _ _ &m0 stat0 ).  apply V_summitup_ll. apply (rewindable_A_plus V). apply rewindable_V_plus. apply D_guess_ll. apply V_summitup_ll.
+apply V_challenge_ll. 
+ progress. 
+
+qed.
+
+
+end section.
